WIP

theories/case_studies/multiuser_kvs/kvs_preamble.v
@@ -16,17 +16,17 @@ Class kvsG Σ :=
       kvs_alloc_genG :: gen_heapGS Z (gset Z) Σ;
     }.
 
-Class kvs_users {Cname : CmptNameG} :=
-  {
-    kvs_users_seals : gmap CmptName Z;
-    kvs_users_seals_dom : forall (C : CmptName), C ∈ dom kvs_users_seals;
-    kvs_users_seals_bounds : ∀ C ku, kvs_users_seals !! C = Some ku -> (0 <= ku < addresses.top)%Z;
+(* Class kvs_users {Cname : CmptNameG} := *)
+(*   { *)
+(*     kvs_users_seals : gmap CmptName Z; *)
+(*     kvs_users_seals_dom : forall (C : CmptName), C ∈ dom kvs_users_seals; *)
+(*     kvs_users_seals_bounds : ∀ C ku, kvs_users_seals !! C = Some ku -> (0 <= ku < addresses.top)%Z; *)
 
-    kvs_users_seals_reserved : list Z;
-    kvs_users_seals_reserved_bounds : Forall (fun k => (0 <= k < addresses.top)%Z) kvs_users_seals_reserved;
+(*     kvs_users_seals_reserved : list Z; *)
+(*     kvs_users_seals_reserved_bounds : Forall (fun k => (0 <= k < addresses.top)%Z) kvs_users_seals_reserved; *)
 
-    kvs_users_seals_unique: NoDup (kvs_users_seals_reserved ++ (map_to_list kvs_users_seals).*2)
-  }.
+(*     kvs_users_seals_unique: NoDup (kvs_users_seals_reserved ++ (map_to_list kvs_users_seals).*2) *)
+(*   }. *)
 
 Definition allocated_keys_auth `{kvsG} ( m : kvs_alloc) : iProp Σ :=
   (gen_heap_interp (L:=Z) (V:= gset Z) m).
@@ -480,7 +480,7 @@ Section KVS_preamble.
     apply elem_of_kvs_map_init in Hk; simplify_eq; iFrame.
   Qed.
 
-  Lemma kvs_initial_map_init (b e : Addr) (init_user_key : Z) :
+  Lemma kvs_initial_map_init (b e : Addr) :
     (b + (ASM_SIZEOF_KVS_ENTRY * SIZE_MAP))%a = Some e ->
     ([[b,e]]↦ₐ[[ kvs_data_kvs_region ]]) -∗
     ([∗ map] idx↦opt_kw ∈ kvs_map_init, idx ⤇(KVS) NONE) -∗
@@ -1175,14 +1175,14 @@ Section KVS_preamble.
     }.
 
   Definition kvs_otype_inv
-    {KVS_layout : kvsLayout} {KVS_users: kvs_users} {KVS_namespaces : kvs_namespaces}
+    {KVS_layout : kvsLayout} {KVS_namespaces : kvs_namespaces}
     (W : WORLD) (C : CmptName) (w : Word) : iProp Σ :=
     ∃ (ku : Z) (a : Addr) (s : gset Z),
       (* Shape of the capability*)
       ⌜ w = WSealable (kvs_user_seal_key_scap Global a) ⌝ ∗
       (* Current address is the user key of the compartment *)
-      ⌜ kvs_users_seals !! C = Some ku ⌝ ∗
       ⌜ (finz.of_z ku) = Some a ⌝ ∗
+      ⌜ (0 <= ku < MAX_USER_KEY)%Z ⌝ ∗
       (* KVS resources *)
       ◯(ALLOC)[ku] s ∗
       ([∗ set] kn ∈ s, ∃ w, (kvs_full_key ku kn) ⤇(KVS) w ∗
@@ -1190,7 +1190,7 @@ Section KVS_preamble.
       ).
 
   Program Definition kvs_otype_prop
-    {KVS_layout : kvsLayout} {KVS_users: kvs_users} {KVS_namespaces : kvs_namespaces} :
+    {KVS_layout : kvsLayout} {KVS_namespaces : kvs_namespaces} :
     (WORLD -n> (leibnizO CmptName) -n> (leibnizO Word) -n> iPropO Σ):=
     λne (W : WORLD) (C : CmptName) (w : Word), (kvs_otype_inv W C w)%I.
   Next Obligation. solve_proper. Defined.
@@ -1198,12 +1198,12 @@ Section KVS_preamble.
   Next Obligation. solve_proper. Defined.
 
   Definition kvs_otype_propC
-    {KVS : kvsLayout} {KVS_users: kvs_users} {KVS_namespaces : kvs_namespaces} :
+    {KVS : kvsLayout} {KVS_namespaces : kvs_namespaces} :
     WORLD * CmptName * leibnizO Word -> iProp Σ :=
     safeC kvs_otype_prop.
 
   Lemma mono_priv_ot_kvs
-    {KVS : kvsLayout} {KVS_users: kvs_users} {KVS_namespaces : kvs_namespaces}
+    {KVS : kvsLayout} {KVS_namespaces : kvs_namespaces}
     (C : CmptName) (w : Word) :
     ⊢ future_priv_mono C kvs_otype_propC w.
   Proof.
@@ -1221,7 +1221,17 @@ Section KVS_preamble.
     by eapply related_sts_priv_trans_world.
   Qed.
 
-  Definition kvs_inv {KVS : kvsLayout} {KVS_users: kvs_users} {KVS_namespaces : kvs_namespaces} : iProp Σ :=
+  Definition seqZ_between (b e : Z) := seqZ b (e-b).
+  Lemma seqZ_between_cons (b e : Z) :
+    (0 < e - b)%Z -> seqZ_between b e = b::(seqZ_between (b+1) e).
+  Proof.
+    intros He.
+    rewrite /seqZ_between seqZ_cons; auto.
+    replace (Z.pred (e - b)) with (e - (b + 1))%Z by lia.
+    done.
+  Qed.
+
+  Definition kvs_inv {KVS : kvsLayout} {KVS_namespaces : kvs_namespaces} : iProp Σ :=
     let imports :=
       kvs_imports b_switcher e_switcher a_switcher_call ot_switcher
     in
@@ -1230,7 +1240,8 @@ Section KVS_preamble.
       (KVS_cgp_b ^+ OFFSET_NEXT_FREE_SEALED_USER_KEY)%a  ↦ₐ (kvs_user_seal_key_scap_init next_free_user_key) ∗
       codefrag KVS_pcc_b' kvs_service_instrs ∗
       isKVS KVS_cgp_b m s ∗
-      ([∗ list] uk ∈ (seqZ next_free_user_key (MemNum-next_free_user_key)), ◯(ALLOC)[uk] ∅) ∗
+      ⌜ (0 <= next_free_user_key <= MAX_USER_KEY)%Z ⌝ ∗
+      ([∗ list] uk ∈ (seqZ_between next_free_user_key MAX_USER_KEY), ◯(ALLOC)[uk] ∅) ∗
       seal_pred KVS_OTYPE kvs_otype_propC.
 
 End KVS_preamble.
