theories/case_studies/multiuser_kvs/kvs_main.v
@@ -11,10 +11,9 @@ Section KVS_Main.
       ```
         #include "kvs.h"
 
-        DECLARE_AND_DEFINE_STATIC_SEALED_VALUE(UserKeyT, service, SealingType, userKey, 1);
-
         void __cheri_compartment("caller1") entry() {
-             auto sealedUserKey = STATIC_SEALED_VALUE(userKey);
+             auto sealedUserKey = initialise();
+             if (!sealedUserKey) { halt; }
              addOrUpdate(sealedUserKey, 1, 12);
              adv.f();
              res = read(sealedUserKey, 1);
@@ -29,12 +28,20 @@ Section KVS_Main.
   Definition KVS_INSERT_OFFSET := 3.
   Definition KVS_READ_OFFSET := 4.
   Definition KVS_ERASE_OFFSET := 5.
-  Definition SEALED_USER_KEY_OFFSET := 6.
+  Definition KVS_INITIALISE_OFFSET := 6.
 
   Definition kvs_main_code : list Word :=
-    fetch_instrs SEALED_USER_KEY_OFFSET cs1 ct0 ct1 (* cs1 -> switcher entry point *)
+    fetch_instrs SWITCHER_CALL_OFFSET ctp ct0 ct1 (* ctp -> switcher entry point *)
+    ++ fetch_instrs KVS_INITIALISE_OFFSET ct1 ct0 cs0  (* ct1 -> {KVS.initialise}_(ot_switcher)  *)
+    ++ encodeInstrsW [ Jalr cra ctp ]
     ++ encodeInstrsW [
-      (* #"main_code"; *)
+      (* if (!sealedUserKey) { halt; } ; *)
+      Jnz 2 ca0; (* ca0 = 0 if initialised. So, jumps not initialised *)
+      Jmp 2;
+      (* Case initialisation failed *)
+      Halt;
+      (* Case initialisation succeeded *)
+      Mov cs1 ca1;
       (* addOrUpdate(sealedUserKey, 1, 12) *)
       Mov ca0 cs1;
       Mov ca1 1;
@@ -85,7 +92,6 @@ Section KVS_Main.
   Definition kvs_main_data  : list Word := [].
 
   Definition kvs_main_imports {KVS : kvsLayout}
-    (KVS_USER_KEY_MAIN : Z)
     (b_switcher e_switcher a_cc_switcher : Addr) (ot_switcher : OType)
     (b_assert e_assert : Addr)
     (B_f : Sealable) : list Word :=
@@ -96,7 +102,7 @@ Section KVS_Main.
       WSealed ot_switcher (KVS_addOrUpdate Global);
       WSealed ot_switcher (KVS_read Global);
       WSealed ot_switcher (KVS_erase Global);
-      (kvs_user_seal_key Global KVS_USER_KEY_MAIN)
+      WSealed ot_switcher (KVS_initialise Global)
     ].
 
 End KVS_Main.
