theories/case_studies/multiuser_kvs/kvs_spec_initialise.v
@@ -17,7 +17,7 @@ Section KVS_spec_initialise.
     {cstackg : CSTACKG Σ}
     `{MP: MachineParameters}
     {swlayout : switcherLayout}
-    {KVS_layout : kvsLayout} {KVS_layout_WF : kvsLayoutWf} {KVS_users: kvs_users} {KVS_namespaces : kvs_namespaces}
+    {KVS_layout : kvsLayout} {KVS_layout_WF : kvsLayoutWf} {KVS_namespaces : kvs_namespaces}
   .
 
   Lemma KVS_initialise_spec_pre
@@ -27,7 +27,7 @@ Section KVS_spec_initialise.
     (next_free_uk : Z)
     :
 
-
+    (0 <= next_free_uk <= MAX_USER_KEY)%Z ->
     SubBounds pc_b pc_e pc_a (pc_a ^+ length kvs_initialise_instrs)%a ->
 
     (cgp_b + length_kvs_data)%a = Some cgp_e ->
@@ -49,16 +49,16 @@ Section KVS_spec_initialise.
       (pc_b ^+ UNSEALING_USER_KEY_OFFSET)%a ↦ₐ kvs_service_unsealing_key ∗
       (cgp_b ^+ OFFSET_NEXT_FREE_SEALED_USER_KEY)%a ↦ₐ (kvs_user_seal_key_scap_init next_free_uk) ∗
 
-      ▷ ([∗ list] uk ∈ (seqZ next_free_uk (MemNum - next_free_uk)%Z), ◯(ALLOC)[uk] ∅) ∗
+      ▷ ([∗ list] uk ∈ (seqZ_between next_free_uk MAX_USER_KEY), ◯(ALLOC)[uk] ∅) ∗
 
       ▷ (PC ↦ᵣ updatePcPerm wret ∗
          cgp ↦ᵣ - ∗
          cra ↦ᵣ - ∗
-         ca0 ↦ᵣ WInt (if ( next_free_uk <? MemNum)%Z then ASM_SOME else ASM_NONE) ∗
+         ca0 ↦ᵣ WInt (if ( next_free_uk <? MAX_USER_KEY)%Z then ASM_TRUE else ASM_FALSE) ∗
          (
-           if ( next_free_uk <? MemNum)%Z
+           if ( next_free_uk <? MAX_USER_KEY)%Z
            then ca1 ↦ᵣ (kvs_user_seal_key Global next_free_uk)
-           else ca1 ↦ᵣ -
+           else ca1 ↦ᵣ WInt 0
          ) ∗ (* result of the initialise *)
          ct0 ↦ᵣ - ∗ (* scratch *)
          ct1 ↦ᵣ - ∗ (* scratch *)
@@ -69,22 +69,22 @@ Section KVS_spec_initialise.
          (pc_b ^+ UNSEALING_USER_KEY_OFFSET)%a ↦ₐ kvs_service_unsealing_key ∗
          (cgp_b ^+ OFFSET_NEXT_FREE_SEALED_USER_KEY)%a ↦ₐ
            (kvs_user_seal_key_scap_init
-              (if ( next_free_uk <? MemNum)%Z
+              (if ( next_free_uk <? MAX_USER_KEY)%Z
                then (next_free_uk + 1)%Z
                else next_free_uk)
            ) ∗
 
          (
-           if ( next_free_uk <? MemNum)%Z
-           then ( ([∗ list] uk ∈ (seqZ (next_free_uk + 1) (MemNum - (next_free_uk + 1))), ◯(ALLOC)[uk] ∅) ∗ ◯(ALLOC)[next_free_uk] ∅)
-           else ([∗ list] uk ∈ (seqZ next_free_uk (MemNum - next_free_uk)%Z), ◯(ALLOC)[uk] ∅)
+           if ( next_free_uk <? MAX_USER_KEY)%Z
+           then ( ([∗ list] uk ∈ (seqZ_between (next_free_uk +1) MAX_USER_KEY), ◯(ALLOC)[uk] ∅) ∗ ◯(ALLOC)[next_free_uk] ∅)
+           else ([∗ list] uk ∈ (seqZ_between next_free_uk MAX_USER_KEY), ◯(ALLOC)[uk] ∅)
          )
 
          -∗ WP Seq (Instr Executable) {{ v, ⌜v = HaltedV⌝ → na_own cerise_nais ⊤ }}
         )
       ⊢ WP Seq (Instr Executable) {{ v, ⌜v = HaltedV⌝ → na_own cerise_nais ⊤ }})%I.
   Proof.
-    iIntros (HsubBounds Hcgp_contiguous)
+    iIntros (Hnext_free_bounds HsubBounds Hcgp_contiguous)
       "(HPC & Hcgp & Hcra & [%wca0 Hca0] & [%wca1 Hca1] & [%wct0 Hct0] & [%wct1 Hct1] & [%wctp Hctp] & [%wcnull Hcnull] & Hcode
       & Ha_unsealing & Ha_next_free_uk & Hnext_free_alloc & Hpost)".
     rewrite /length_kvs_data /= in Hcgp_contiguous.
@@ -115,19 +115,37 @@ Section KVS_spec_initialise.
     iInstr "Hcode".
     (* lt ctp ctp MemNum; (* ctp := if (ctp < MemNum) then 1 else 0 *) *)
     iInstr "Hcode".
+    Transparent MemNum.
+    replace 1999999%Z with MAX_USER_KEY.
+    2: { rewrite /MAX_USER_KEY /MemNum; lia. }
 
-    destruct ( ((0 ^+ next_free_uk)%a <? 2000000)%Z ) eqn:Hnext_free_uk; iEval (cbn) in "Hctp".
+    destruct ( ((0 ^+ next_free_uk)%a <? MAX_USER_KEY)%Z ) eqn:Hnext_free_uk; iEval (cbn) in "Hctp".
     - apply Z.ltb_lt in Hnext_free_uk.
-      assert ( (next_free_uk <? MemNum)%Z = true ) as Hnext_free_uk_true.
-      { Transparent MemNum.
-        rewrite /MemNum.
+      assert ( (next_free_uk <? MAX_USER_KEY)%Z = true ) as Hnext_free_uk_true.
+      {
         apply Z.ltb_lt.
-        admit.
+        rewrite /MAX_USER_KEY /MemNum.
+        rewrite /MAX_USER_KEY {5}/MemNum in Hnext_free_uk.
+        replace (2000000 - 1)%Z with 1999999%Z by lia.
+        replace (2000000 - 1)%Z with 1999999%Z in Hnext_free_uk by lia.
+        clear -Hnext_free_bounds Hnext_free_uk.
+        Set Printing Coercions.
+        rewrite /z_of in Hnext_free_uk.
+        rewrite /finz.incr_default in Hnext_free_uk.
+        rewrite /finz.incr in Hnext_free_uk.
+        destruct ( Z.lt_dec (z_of 0%a + next_free_uk)%Z MemNum ) eqn:H1; try solve_addr.
+        - admit.
+        - admit.
+          destruct (Z.le_dec 0 (z_of 0%a + next_free_uk)%Z) eqn:H2; try solve_addr.
+        destruct ( (0 + next_free_uk)%a ) eqn:H.
+        destruct next_free_uk; try lia
+        destruct ( (0 + next_free_uk)%a ) eqn:H; try solve_addr.
+        destruct ( finz.largest 0%a ) eqn:H'; try solve_addr.
       }
       rewrite Hnext_free_uk_true.
       (* jnz (".initialise_next_free_available")%asm ctp; *)
       iInstr "Hcode".
-      (* mov ca0 ASM_SOME; *)
+      (* mov ca0 ASM_TRUE; *)
       iInstr "Hcode".
       (* seal ca1 ct0 ct1; *)
       iInstr "Hcode"; auto.
@@ -135,7 +153,10 @@ Section KVS_spec_initialise.
       (* lea ct1 1; *)
       iInstr "Hcode".
       { transitivity (Some (0 ^+ (next_free_uk + 1)%Z)%a); auto.
-        admit.
+        apply Z.ltb_lt in Hnext_free_uk_true.
+        assert ( (z_of (0 ^+ next_free_uk)%a < MemNum)%Z ).
+        { solve_addr. }
+        solve_addr.
       }
       (* store cgp ct1; *)
       iInstr_lookup "Hcode" as "Hi" "Hcode".
@@ -156,7 +177,6 @@ Section KVS_spec_initialise.
       { iDestruct "Hnext_free_alloc" as "[$ H]".
         by replace ( (Z.pred (MemNum - next_free_uk)) ) with (MemNum - (next_free_uk + 1))%Z by lia.
       }
-      Transparent MemNum.
       rewrite /MemNum.
       rewrite /MemNum in Hnext_free_uk_true.
       apply Z.ltb_lt in Hnext_free_uk_true.
@@ -164,14 +184,18 @@ Section KVS_spec_initialise.
 
     - apply Z.ltb_ge in Hnext_free_uk.
       assert ( (next_free_uk <? MemNum)%Z = false ) as ->.
-      { Transparent MemNum.
+      {
         rewrite /MemNum.
         apply Z.ltb_ge.
+        lia.
+        solve_addr.
         admit.
       }
       (* jnz (".initialise_next_free_available")%asm ctp; *)
       iInstr "Hcode".
-      (* mov ca0 ASM_NONE; *)
+      (* mov ca0 ASM_FALSE; *)
+      iInstr "Hcode".
+      (* mov ca1 0; *)
       iInstr "Hcode".
       (* ret; *)
       iInstr "Hcode".
@@ -181,7 +205,7 @@ Section KVS_spec_initialise.
       iFrame "HPC Hcgp Hcra Hca0 Hca1 Hct1 Hct0 Hctp Hcnull Hcode Ha_unsealing Ha_next_free_uk Hnext_free_alloc".
   Admitted.
 
-  Lemma KVS_initialise_spec_in
+  Lemma KVS_initialise_spec
     (wret : Word)
     (E : coPset)
     :
@@ -212,14 +236,14 @@ Section KVS_spec_initialise.
          cnull ↦ᵣ - ∗
          (
            ( ∃ next_free_uk,
-               ⌜ (next_free_uk <? MemNum)%Z ⌝ ∗
-               ca0 ↦ᵣ WInt ASM_SOME ∗
+               ⌜ (0 <= next_free_uk < MemNum)%Z ⌝ ∗
+               ca0 ↦ᵣ WInt ASM_TRUE ∗
                ca1 ↦ᵣ (kvs_user_seal_key Global next_free_uk) ∗
                ◯(ALLOC)[next_free_uk] ∅
            )
            ∨
              (
-               ca0 ↦ᵣ WInt ASM_NONE ∗
+               ca0 ↦ᵣ WInt ASM_FALSE ∗
                ca1 ↦ᵣ -
              )
          )
@@ -231,7 +255,8 @@ Section KVS_spec_initialise.
     iIntros (Hnkvs_E)
       "(#Hkvs_inv & Hna & HPC & Hcgp & Hcra & Hca0 & Hca1 & Hct0 & Hct1 & Hctp & Hcnull & Hpost)".
     iMod (na_inv_acc with "Hkvs_inv Hna")
-      as "( (%m & %s & %next_free_uk & >Himports & >Hcgp_e & >Hcode & HisKVS & Hfree_uk_alloc & #Hspred) & Hna & Hkvs_inv_close)"; eauto.
+      as "( (%m & %s & %next_free_uk & >Himports & >Hcgp_e & >Hcode
+            & HisKVS & >%Hwf_free_uk & Hfree_uk_alloc & #Hspred) & Hna & Hkvs_inv_close)"; eauto.
     pose proof (Hcgp_continuous := KVS_size_data).
     pose proof (HKVS_pcc_b' := KVS_size_imports).
     pose proof (Hcode_continuous := KVS_size_code).
@@ -256,17 +281,22 @@ Section KVS_spec_initialise.
 
     destruct ( (next_free_uk <? MemNum)%Z ) eqn:Hfree.
     - iDestruct "Hfree_uk_alloc" as "[Hfree_uk_alloc Halloc]".
+      assert (0 <= next_free_uk + 1 <= MemNum )%Z by (apply Z.ltb_lt in Hfree; lia).
       iMod ("Hkvs_inv_close" with "[$Hcode $Hcgp_e Himports_sw Ha_unsealing $HisKVS $Hfree_uk_alloc $Hspred $Hna]") as "Hna" ; auto.
       { iNext.
+        iSplit; last done.
         iApply (region_pointsto_cons with "[Ha_unsealing Himports_sw]"); eauto; iFrame.
         iApply (region_pointsto_cons with "[Ha_unsealing]"); eauto; [solve_addr+|]; iFrame.
         rewrite /region_pointsto finz_seq_between_empty; auto; solve_addr+.
       }
       iApply "Hpost"; iFrame.
       iLeft; iFrame.
-      iPureIntro; rewrite Hfree; auto.
+      iPureIntro; auto.
+      apply Z.ltb_lt in Hfree.
+      lia.
     - iMod ("Hkvs_inv_close" with "[$Hcode $Hcgp_e Himports_sw Ha_unsealing $HisKVS $Hfree_uk_alloc $Hspred $Hna]") as "Hna" ; auto.
       { iNext.
+        iSplit; last done.
         iApply (region_pointsto_cons with "[Ha_unsealing Himports_sw]"); eauto; iFrame.
         iApply (region_pointsto_cons with "[Ha_unsealing]"); eauto; [solve_addr+|]; iFrame.
         rewrite /region_pointsto finz_seq_between_empty; auto; solve_addr+.
